

3

1. First, since $\{\alpha\}_{i=1}^n, \{\beta\}_{i=1}^n$ are orthonormal set, as we studied in class it means that:

$$\int_0^1 \alpha_i(t) \alpha_j(t) dt = \delta_{ij}$$

$$\int_0^1 \beta_i(t) \beta_j(t) dt = \delta_{ij}$$

As for the set $\psi_i(t) = \frac{1}{\sqrt{2}} \begin{bmatrix} \alpha_i(t) \\ \beta_i(t) \end{bmatrix}$, first we will prove they are normalized using the inner-product defined in the question:

$$\langle \psi_i, \psi_i \rangle = \int_0^1 \left(\frac{1}{\sqrt{2}} \alpha_i(t) \frac{1}{\sqrt{2}} \alpha_i(t) + \frac{1}{\sqrt{2}} \beta_i(t) \frac{1}{\sqrt{2}} \beta_i(t) \right) dt$$

$$\frac{1}{2} \int_0^1 \alpha_i(t) \alpha_i(t) dt + \frac{1}{2} \int_0^1 \beta_i(t) \beta_i(t) dt =_{(1)} \frac{1}{2} \cdot 1 + \frac{1}{2} \cdot 1 = 1$$

Explanations:

(1) : We used the orthogonality of $\{\alpha\}_{i=1}^n, \{\beta\}_{i=1}^n$ which means:

$$\int_0^1 \alpha_i(t) \alpha_i(t) dt = 1$$

$$\int_0^1 \beta_i(t) \beta_i(t) dt = 1$$

Now we prove they are orthogonal, for $i \neq j$:

$$\langle \psi_i, \psi_j \rangle = \int_0^1 \left(\frac{1}{\sqrt{2}} \alpha_i(t) \frac{1}{\sqrt{2}} \alpha_j(t) + \frac{1}{\sqrt{2}} \beta_i(t) \frac{1}{\sqrt{2}} \beta_j(t) \right) dt$$

$$\frac{1}{2} \int_0^1 \alpha_i(t) \alpha_j(t) dt + \frac{1}{2} \int_0^1 \beta_i(t) \beta_j(t) dt =_{(1)} \frac{1}{2} \cdot 0 + \frac{1}{2} \cdot 0 = 0$$

Explanations:

(1) : We used the orthogonality of $\{\alpha\}_{i=1}^n, \{\beta\}_{i=1}^n$ which means:

$$\int_0^1 \alpha_i(t) \alpha_j(t) dt = 0$$

$$\int_0^1 \beta_i(t) \beta_j(t) dt = 0$$

2. $\psi_i(t) : [0, 1) \rightarrow \mathbb{R}^2, \phi(t) : [0, 1) \rightarrow \mathbb{R}^2$, therefore we can define $\psi_i(t) \triangleq \begin{bmatrix} \psi_i^1(t) \\ \psi_i^2(t) \end{bmatrix}, \phi(t) \triangleq \begin{bmatrix} \phi^1(t) \\ \phi^2(t) \end{bmatrix}$, than:

$$\tilde{\phi}(t) = \sum_{i=1}^N \phi_i \psi_i(t) = \sum_{i=1}^N \phi_i \begin{bmatrix} \psi_i^1(t) \\ \psi_i^2(t) \end{bmatrix} = \begin{bmatrix} \sum_{i=1}^N \phi_i \psi_i^1(t) \\ \sum_{i=1}^N \phi_i \psi_i^2(t) \end{bmatrix}$$

now we use this expression in order to calculate the error:

$$\phi(t) - \tilde{\phi}(t) = \begin{bmatrix} \phi^1(t) \\ \phi^2(t) \end{bmatrix} - \begin{bmatrix} \sum_{i=1}^N \phi_i \psi_i^1(t) \\ \sum_{i=1}^N \phi_i \psi_i^2(t) \end{bmatrix} = \begin{bmatrix} \phi^1(t) - \sum_{i=1}^N \phi_i \psi_i^1(t) \\ \phi^2(t) - \sum_{i=1}^N \phi_i \psi_i^2(t) \end{bmatrix}$$

and the approximation MSE is:

$$\begin{aligned} MSE &= \left\langle \phi(t) - \tilde{\phi}(t), \phi(t) - \tilde{\phi}(t) \right\rangle \\ &= \left\langle \begin{bmatrix} \phi^1(t) - \sum_{i=1}^N \phi_i \psi_i^1(t) \\ \phi^2(t) - \sum_{i=1}^N \phi_i \psi_i^2(t) \end{bmatrix}, \begin{bmatrix} \phi^1(t) - \sum_{i=1}^N \phi_i \psi_i^1(t) \\ \phi^2(t) - \sum_{i=1}^N \phi_i \psi_i^2(t) \end{bmatrix} \right\rangle \\ &= \int_0^1 \left(\left(\phi^1(t) - \sum_{i=1}^N \phi_i \psi_i^1(t) \right)^2 + \left(\phi^2(t) - \sum_{i=1}^N \phi_i \psi_i^2(t) \right)^2 \right) dt \\ &= \int_0^1 \left(\phi^1(t) - \sum_{i=1}^N \phi_i \psi_i^1(t) \right)^2 dt + \int_0^1 \left(\phi^2(t) - \sum_{i=1}^N \phi_i \psi_i^2(t) \right)^2 dt \end{aligned}$$

The optimal coefficients in MSE sense will achived by demending:

$$\frac{\partial MSE}{\partial \phi_j} = 0$$

Lets calculate the derivative:

$$\begin{aligned} \frac{\partial MSE}{\partial \phi_j} &= \frac{\partial}{\partial \phi_j} \int_0^1 \left(\phi^1(t) - \sum_{i=1}^N \phi_i \psi_i^1(t) \right)^2 dt + \frac{\partial}{\partial \phi_j} \int_0^1 \left(\phi^2(t) - \sum_{i=1}^N \phi_i \psi_i^2(t) \right)^2 dt \\ &= \int_0^1 \frac{\partial}{\partial \phi_j} \left(\phi^1(t) - \sum_{i=1}^N \phi_i \psi_i^1(t) \right)^2 dt + \int_0^1 \frac{\partial}{\partial \phi_j} \left(\phi^2(t) - \sum_{i=1}^N \phi_i \psi_i^2(t) \right)^2 dt \\ &= -2 \int_0^1 \psi_j^1(t) \left(\phi^1(t) - \sum_{i=1}^N \phi_i \psi_i^1(t) \right) dt - 2 \int_0^1 \psi_j^2(t) \left(\phi^2(t) - \sum_{i=1}^N \phi_i \psi_i^2(t) \right) dt \end{aligned}$$

$$\begin{aligned}
&= -2 \int_0^1 \psi_j^1(t) \phi^1(t) dt + 2 \sum_{i=1}^N \phi_i \int_0^1 \psi_j^1(t) \psi_i^1(t) dt - 2 \int_0^1 \psi_j^2(t) \phi^2(t) dt + 2 \sum_{i=1}^N \phi_i \int_0^1 \psi_j^2(t) \psi_i^2(t) dt \\
&\quad - 2 \int_0^1 \psi_j^1(t) \phi^1(t) dt - 2 \int_0^1 \psi_j^2(t) \phi^2(t) dt + 2 \sum_{i=1}^N \phi_i \left(\int_0^1 \psi_j^1(t) \psi_i^1(t) dt + \int_0^1 \psi_j^2(t) \psi_i^2(t) dt \right) \\
&\quad =_{(1)} -2 \int_0^1 \psi_j^1(t) \phi^1(t) dt - 2 \int_0^1 \psi_j^2(t) \phi^2(t) dt + 2 \phi_j
\end{aligned}$$

(1) : $\psi_i(t) : [0, 1] \rightarrow \mathbb{R}^2$ is orthonormal set and therefore:

$$\int_0^1 \psi_j^1(t) \psi_i^1(t) dt + \int_0^1 \psi_j^2(t) \psi_i^2(t) dt = \delta_{ij}$$

Now lets demand $\frac{\partial MSE}{\partial \phi_j} = 0$ and we get:

$$\phi_j^{opt} = \int_0^1 \psi_j^1(t) \phi^1(t) dt + \int_0^1 \psi_j^2(t) \phi^2(t) dt = \langle \psi_j, \phi(t) \rangle$$

for $j = 1, \dots, N$

Now lets calculate expression for minimal approximation MSE:

$$\begin{aligned}
MSE_{opt} &= \int_0^1 \left(\phi^1(t) - \sum_{i=1}^N \phi_i^{opt} \psi_i^1(t) \right)^2 dt + \int_0^1 \left(\phi^2(t) - \sum_{i=1}^N \phi_i^{opt} \psi_i^2(t) \right)^2 dt \\
&= \int_0^1 (\phi^1(t))^2 - 2 \int_0^1 \phi^1(t) \sum_{i=1}^N \phi_i^{opt} \psi_i^1(t) dt + \int_0^1 \left(\sum_{i=1}^N \phi_i^{opt} \psi_i^1(t) \right)^2 dt \\
&\quad + \int_0^1 (\phi^2(t))^2 - 2 \int_0^1 \phi^2(t) \sum_{i=1}^N \phi_i^{opt} \psi_i^2(t) dt + \int_0^1 \left(\sum_{i=1}^N \phi_i^{opt} \psi_i^2(t) \right)^2 dt \\
&= \int_0^1 (\phi^1(t))^2 - 2 \sum_{i=1}^N \phi_i^{opt} \int_0^1 \phi^1(t) \psi_i^1(t) dt + \sum_{i=1}^N \sum_{j=1}^N \phi_i^{opt} \phi_j^{opt} \int_0^1 \psi_i^1(t) \psi_j^1(t) dt \\
&\quad + \int_0^1 (\phi^2(t))^2 - 2 \sum_{i=1}^N \phi_i^{opt} \int_0^1 \phi^2(t) \psi_i^2(t) dt + \sum_{i=1}^N \sum_{j=1}^N \phi_i^{opt} \phi_j^{opt} \int_0^1 \psi_i^2(t) \psi_j^2(t) dt \\
&= \int_0^1 (\phi^1(t))^2 + \int_0^1 (\phi^2(t))^2 - 2 \sum_{i=1}^N \phi_i^{opt} \left(\int_0^1 \phi^1(t) \psi_i^1(t) dt + \int_0^1 \phi^2(t) \psi_i^2(t) dt \right) \\
&\quad + \sum_{i=1}^N \sum_{j=1}^N \phi_i^{opt} \phi_j^{opt} \left(\int_0^1 \psi_i^1(t) \psi_j^1(t) dt + \int_0^1 \psi_i^2(t) \psi_j^2(t) dt \right)
\end{aligned}$$

$$\begin{aligned}
&=_{(1)} \int_0^1 (\phi^1(t))^2 + \int_0^1 (\phi^2(t))^2 - 2 \sum_{i=1}^N (\phi_i^{opt})^2 + \sum_{i=1}^N (\phi_i^{opt})^2 \\
&= \int_0^1 (\phi^1(t))^2 + \int_0^1 (\phi^2(t))^2 - \sum_{i=1}^N (\phi_i^{opt})^2
\end{aligned}$$

Explanations:

(1) :As we showed : $\int_0^1 \phi^1(t)\psi_i^1(t)dt + \int_0^1 \phi^2(t)\psi_i^2(t)dt = \phi_i^{opt}$, and by inner-product definition:

$$\int_0^1 \psi_i^1(t)\psi_j^1(t)dt + \int_0^1 \psi_i^2(t)\psi_j^2(t)dt = \delta_{ij}$$

And by the given definition for inner-product we can write the expression we got as:

$$MSE_{opt} = \langle \phi(t), \phi(t) \rangle - \sum_{i=1}^N (\phi_i^{opt})^2$$